simplify reasoning about MemI.cas using lemmas about MemI.load & MemI.store

imp_system/mem/MemI.v
@@ -5,6 +5,120 @@ Require Export MemHeader.
 Set Implicit Arguments.
 Set Typeclasses Depth 5.
 
+Module Mem.
+
+  (* Definition t : Type := mblock -> option (Z -> val). *)
+  Record t : Type := mk {
+    cnts : mblock -> Z -> option val;
+    nb : mblock;
+    (*** Q : wf conditions like nextmblock_noaccess ? ***)
+    (*** A : Unlike in CompCert, the memory object will not float in various places in the program.
+            It suffices to state wf only inside Mem module. (probably by utilizing URA.wf)
+     ***)
+  }
+  .
+
+  Definition wf (m0 : t) : Prop := forall blk ofs (LT : (blk < m0.(nb))%nat), m0.(cnts) blk ofs = None.
+
+  Definition alloc (m0 : Mem.t) (sz : Z) : (mblock * Mem.t) :=
+    ((m0.(nb)),
+     Mem.mk (update (m0.(cnts)) (m0.(nb))
+                    (fun ofs => if (0 <=? ofs)%Z && (ofs <? sz)%Z then Some (Vundef) else None))
+            (S m0.(nb))
+    )
+  .
+
+  Opaque Z.ltb Z.leb Z.mul Z.eq_dec Nat.eq_dec.
+  (* Definition empty : t := mk (update (fun _ _ => None) 0 (fun ofs => if dec ofs 0%Z then Some Vundef else None)) 0. *)
+  Definition empty : t := mk (fun _ _ => None) 0.
+  (* Let empty2 : t := Eval compute in *)
+  (*   let m0 := mk (fun _ _ => None) 0 in *)
+  (*   let (_, m1) := alloc m0 1%Z in *)
+  (*   m1 *)
+  (* . *)
+  (*** shoul allocated with Vundef, not 0 ***)
+
+  (*** TODO : Unlike CompCert, this "free" function does not take offset.
+       In order to support this, we need more sophisticated RA. it would be interesting.
+   ***)
+  (* Definition free (m0 : Mem.t) (b : mblock) : option (Mem.t) := *)
+  (*   match m0.(cnts) b ofs0 with *)
+  (*   | Some _ => Some (Mem.mk (update m0.(cnts) b (fun _ => None)) m0.(nb)) *)
+  (*   | _ => None *)
+  (*   end *)
+  (* . *)
+
+  Definition free (m0 : Mem.t) := fun '(b,ofs) =>
+    match m0.(cnts) b ofs with
+    | Some _ => Some (Mem.mk (update m0.(cnts) b (update (m0.(cnts) b) ofs None)) m0.(nb))
+    | _ => None
+    end
+  .
+
+  Definition load (m0 : Mem.t) := fun '(b,ofs) =>
+    m0.(cnts) b ofs.
+
+  Definition store (m0 : Mem.t) := fun '(b,ofs) v =>
+    match m0.(cnts) b ofs with
+    | Some _ => Some (Mem.mk (fun _b _ofs => if (dec b _b) && (dec ofs _ofs)
+                                             then Some v
+                                             else m0.(cnts) _b _ofs) m0.(nb))
+    | _ => None
+    end
+  .
+
+  Definition valid_ptr (m0 : Mem.t) := fun '(b,ofs) =>
+    is_some (m0.(cnts) b ofs).
+
+(*** NOTE : Probably we can support comparison between nullptr and 0 ***)
+(*** NOTE : Unlike CompCert, we don't support comparison with weak_valid_ptr (for simplicity) ***)
+
+  Definition load_mem (csl : string -> bool) (genv : GEnv.t) : Mem.t :=
+    Mem.mk
+      (fun blk ofs =>
+         do '(g, gd) <- (List.nth_error genv blk);
+         match gd↓ with
+         | Some Gfun =>
+           None
+         | Some (Gvar gv) =>
+           if csl g then None else
+           if (dec ofs 0%Z) then Some (Vint gv) else None
+          | _ => None
+         end)
+      (*** TODO : This simplified model doesn't allow function pointer comparsion.
+           To be more faithful, we need to migrate the notion of "permission" from CompCert.
+           CompCert expresses it with "nonempty" permission.
+       ***)
+      (*** TODO : When doing so, I would like to extend val with "Vfid (id : string)" case.
+           That way, I might be able to support more higher-order features (overriding, newly allocating function)
+       ***)
+      (List.length genv)
+  .
+
+  Definition mem_pad (m0 : Mem.t) (delta : nat) : Mem.t :=
+    Mem.mk m0.(Mem.cnts) (m0.(Mem.nb) + delta)
+  .
+
+  Definition vcmp (m0 : Mem.t) (x y : val) : option bool :=
+    match x, y with
+    | Vint x, Vint y => Some (dec x y : bool)
+    | Vptr (x, xofs), Vptr (y, yofs) =>
+      if Mem.valid_ptr m0 (x, xofs) && Mem.valid_ptr m0 (y, yofs)
+      then Some (dec x y && dec xofs yofs)
+      else None
+    | Vptr (x, xofs), Vint y =>
+      if Mem.valid_ptr m0 (x, xofs) && dec y 0%Z
+      then Some false
+      else None
+    | Vint x, Vptr (y, yofs) =>
+      if Mem.valid_ptr m0 (y, yofs) && dec x 0%Z
+      then Some false
+      else None
+    | _, _ => None
+    end.
+
+End Mem.
+
 Module MemI. Section MemI.
   Context {Σ: GRA}.
 
@@ -26,37 +140,36 @@ Module MemI. Section MemI.
 
   Definition free : list val → itree pmodE val :=
     λ varg,
-      '(b, ofs): (nat * Z) <- (pargs [Tptr] varg)?;;
+      bofs <- (pargs [Tptr] varg)?;;
       mem <- trigger (SGet v_mem);; mem <- mem↓?;;
-      mem1 <- (Mem.free mem b ofs)?;;
+      mem1 <- (Mem.free mem bofs)?;;
       trigger (SPut v_mem mem1↑);;;
       Ret (Vint 0)
   . 
 
   Definition load: list val -> itree pmodE val :=
     fun varg =>      
-      '(b, ofs): (nat * Z) <- (pargs [Tptr] varg)?;;        
+      bofs <- (pargs [Tptr] varg)?;;        
       mem <- trigger (SGet v_mem);; mem <- mem↓?;;
-      v <- (Mem.load mem b ofs)?;;
+      v <- (Mem.load mem bofs)?;;
       Ret v
   .
 
   Definition store : list val → itree pmodE val :=
     fun varg =>
-      '(b, ofs, v): (nat * Z * val) <- (pargs [Tptr; Tuntyped] varg)?;;
+      '(bofs, v): _ <- (pargs [Tptr; Tuntyped] varg)?;;
       mem <- trigger (SGet v_mem);; mem <- mem↓?;;
-      mem1 <- (Mem.store mem b ofs v)?;;
+      mem1 <- (Mem.store mem bofs v)?;;
       trigger (SPut v_mem mem1↑);;;
       Ret (Vint 0)
   .
 
   Definition cmp : list val → itree pmodE val :=
     fun varg =>
-      '(v0, v1): (val * val) <- (pargs [Tuntyped; Tuntyped] varg)?;;
-      '(v0, v1): (val * val) <- (pargs [Tuntyped; Tuntyped] varg)?;;
+      '(v0, v1): _ <- (pargs [Tuntyped; Tuntyped] varg)?;;
       mem <- trigger (SGet v_mem);; mem <- mem↓?;;
-      b <- (vcmp mem v0 v1)?;;
-      if b: bool
+      'b: bool <- (Mem.vcmp mem v0 v1)?;;
+      if b
       then 
         Ret (Vint 1%Z)
       else
@@ -65,13 +178,11 @@ Module MemI. Section MemI.
 
   Definition cas: list val -> itree pmodE val :=
     fun varg =>
-     ' (b, ofs, (v_old, v_new)): (nat * Z * (val * val)) <- (pargs [Tptr; Tuntyped; Tuntyped] varg)?;;        
-      mem <- trigger (SGet v_mem);; mem <- mem↓?;;
-      d <- (Mem.load mem b ofs)?;;
+      ' (bofs, (v_old, v_new)): _ <- (pargs [Tptr; Tuntyped; Tuntyped] varg)?;;
+      'd: val <- ccallU MemHdr.load [Vptr bofs];;
       if (dec d v_old)
       then
-        mem1 <- (Mem.store mem b ofs v_new)?;;
-        _ <- trigger (SPut v_mem mem1↑);;
+        '_: val <- ccallU MemHdr.store [Vptr bofs; v_new];;
         Ret d
       else
         Ret d
